theories/zoo/prelude/prelude.v
@@ -3,3 +3,16 @@ From zoo.prelude Require Export
   tactics.
 
 Coercion Z.of_nat : nat >-> Z.
+
+Notation "₊ n" := (
+  Z.to_nat n
+)(at level 3,
+  right associativity,
+  format "₊ n"
+) : stdpp_scope.
+Notation "⁺ n" := (
+  Z.of_nat n
+)(at level 3,
+  right associativity,
+  format "⁺ n"
+) : stdpp_scope.
