theories/zoo_std/dynarray_1.v
@@ -77,7 +77,7 @@ Section zoo_G.
       dynarray_1_make #sz v
     {{{ t,
       RET t;
-      dynarray_1_model t (replicate (Z.to_nat sz) v)
+      dynarray_1_model t (replicate ₊sz v)
     }}}.
   Proof.
     iIntros "% %Φ _ HΦ".
@@ -95,7 +95,7 @@ Section zoo_G.
       ▷ Ψ 0 [] ∗
       □ (
         ∀ i vs,
-        ⌜i < Z.to_nat sz ∧ i = length vs⌝ -∗
+        ⌜i < ₊sz ∧ i = length vs⌝ -∗
         Ψ i vs -∗
         WP fn #i {{ v,
           ▷ Ψ (S i) (vs ++ [v])
@@ -105,9 +105,9 @@ Section zoo_G.
       dynarray_1_initi #sz fn
     {{{ t vs,
       RET t;
-      ⌜length vs = Z.to_nat sz⌝ ∗
+      ⌜length vs = ₊sz⌝ ∗
       dynarray_1_model t vs ∗
-      Ψ (Z.to_nat sz) vs
+      Ψ ₊sz vs
     }}}.
   Proof.
     iIntros "%Hsz %Φ (HΨ & #Hfn) HΦ".
@@ -120,7 +120,7 @@ Section zoo_G.
     (0 ≤ sz)%Z →
     {{{
       ▷ Ψ 0 [] ∗
-      ( [∗ list] i ∈ seq 0 (Z.to_nat sz),
+      ( [∗ list] i ∈ seq 0 ₊sz,
         ∀ vs,
         ⌜i = length vs⌝ -∗
         Ψ i vs -∗
@@ -132,20 +132,20 @@ Section zoo_G.
       dynarray_1_initi #sz fn
     {{{ t vs,
       RET t;
-      ⌜length vs = Z.to_nat sz⌝ ∗
+      ⌜length vs = ₊sz⌝ ∗
       dynarray_1_model t vs ∗
-      Ψ (Z.to_nat sz) vs
+      Ψ ₊sz vs
     }}}.
   Proof.
     iIntros "%Hsz %Φ (HΨ & Hfn) HΦ".
     match goal with |- context [big_opL bi_sep (λ _, ?Ξ') _] => set Ξ := Ξ' end.
     pose (Ψ' i vs := (
       Ψ i vs ∗
-      [∗ list] j ∈ seq i (Z.to_nat sz - i), Ξ j
+      [∗ list] j ∈ seq i (₊sz - i), Ξ j
     )%I).
     wp_apply (dynarray_1_initi_spec Ψ' with "[$HΨ Hfn]"); [done | | iSteps].
     rewrite Nat.sub_0_r. iFrame. iIntros "!> %i %vs (%Hi1 & %Hi2) (HΨ & HΞ)".
-    destruct (Nat.lt_exists_pred 0 (Z.to_nat sz - i)) as (k & Hk & _); first lia. rewrite Hk.
+    destruct (Nat.lt_exists_pred 0 (₊sz - i)) as (k & Hk & _); first lia. rewrite Hk.
     rewrite -cons_seq. iDestruct "HΞ" as "(Hfn & HΞ)".
     wp_apply (wp_wand with "(Hfn [//] HΨ)").
     iSteps. rewrite Nat.sub_succ_r Hk //.
@@ -155,7 +155,7 @@ Section zoo_G.
     {{{
       □ (
         ∀ i,
-        ⌜i < Z.to_nat sz⌝ -∗
+        ⌜i < ₊sz⌝ -∗
         WP fn #i {{ v,
           ▷ Ψ i v
         }}
@@ -164,7 +164,7 @@ Section zoo_G.
       dynarray_1_initi #sz fn
     {{{ t vs,
       RET t;
-      ⌜length vs = Z.to_nat sz⌝ ∗
+      ⌜length vs = ₊sz⌝ ∗
       dynarray_1_model t vs ∗
       ( [∗ list] i ↦ v ∈ vs,
         Ψ i v
@@ -182,7 +182,7 @@ Section zoo_G.
   Lemma dynarray_1_initi_spec_disentangled' Ψ sz fn :
     (0 ≤ sz)%Z →
     {{{
-      ( [∗ list] i ∈ seq 0 (Z.to_nat sz),
+      ( [∗ list] i ∈ seq 0 ₊sz,
         WP fn #i {{ v,
           ▷ Ψ i v
         }}
@@ -191,7 +191,7 @@ Section zoo_G.
       dynarray_1_initi #sz fn
     {{{ t vs,
       RET t;
-      ⌜length vs = Z.to_nat sz⌝ ∗
+      ⌜length vs = ₊sz⌝ ∗
       dynarray_1_model t vs ∗
       ( [∗ list] i ↦ v ∈ vs,
         Ψ i v
@@ -257,7 +257,7 @@ Section zoo_G.
 
   Lemma dynarray_1_get_spec t vs (i : Z) v :
     (0 ≤ i)%Z →
-    vs !! Z.to_nat i = Some v →
+    vs !! ₊i = Some v →
     {{{
       dynarray_1_model t vs
     }}}
@@ -282,7 +282,7 @@ Section zoo_G.
       dynarray_1_set t #i v
     {{{
       RET ();
-      dynarray_1_model t (<[Z.to_nat i := v]> vs)
+      dynarray_1_model t (<[₊i := v]> vs)
     }}}.
   Proof.
     iIntros "%Hi %Φ (:model) HΦ".
@@ -314,7 +314,7 @@ Section zoo_G.
       dynarray_1_reserve #l #n
     {{{ data' extra',
       RET ();
-      ⌜Z.to_nat n ≤ length vs + extra'⌝ ∗
+      ⌜₊n ≤ length vs + extra'⌝ ∗
       model' l (length vs) data' (vs ++ replicate extra' ()%V)
     }}}.
   Proof.
@@ -331,7 +331,7 @@ Section zoo_G.
       { rewrite length_app. lia. }
       { rewrite length_replicate. lia. }
       wp_store.
-      iApply ("HΦ" $! data' (Z.to_nat (n `max` n') - length vs)).
+      iApply ("HΦ" $! data' (₊(n `max` n') - length vs)).
       iSteps. rewrite Nat2Z.id drop_replicate take_app_length //.
     - iApply ("HΦ" $! data extra).
       iSteps.
@@ -359,7 +359,7 @@ Section zoo_G.
       dynarray_1_reserve_extra #l #n
     {{{ data' extra',
       RET ();
-      ⌜Z.to_nat n ≤ extra'⌝ ∗
+      ⌜₊n ≤ extra'⌝ ∗
       model' l (length vs) data' (vs ++ replicate extra' ()%V)
     }}}.
   Proof.
